<?xml version="1.0"?>
<rdf:RDF xmlns="http://www.example.org/dqa#"
     xml:base="http://www.example.org/dqa"
     xmlns:dqv="http://www.w3.org/ns/dqv#"
     xmlns:owl="http://www.w3.org/2002/07/owl#"
     xmlns:rdf="http://www.w3.org/1999/02/22-rdf-syntax-ns#"
     xmlns:xml="http://www.w3.org/XML/1998/namespace"
     xmlns:xsd="http://www.w3.org/2001/XMLSchema#"
     xmlns:foaf="http://xmlns.com/foaf/0.1/"
     xmlns:rdfs="http://www.w3.org/2000/01/rdf-schema#"
     xmlns:skos="http://www.w3.org/2004/02/skos/core#"
     xmlns:vann="http://purl.org/vocab/vann/"
     xmlns:terms="http://purl.org/dc/terms/">
    <owl:Ontology rdf:about="http://www.example.org/dqa">
        <owl:versionIRI rdf:resource="http://www.example.org/dqa/1.0.0"/>
        <owl:imports rdf:resource="http://www.w3.org/ns/dqv#"/>
        <terms:created rdf:datatype="http://www.w3.org/2001/XMLSchema#date">2025-02-04</terms:created>
        <terms:creator>https://www.linkedin.com/in/oumaima-amal/</terms:creator>
        <terms:description>DQA : an extension of the DQV ontology designed to enhance the assessment of data quality by introducing structured evaluation processes, traceability of applied methods, and granularities and also results of indicators application. It extends DQV by incorporating assessment processes, granular evaluation levels, formula-based and path-based assessment methods, and qualitative labels for evaluation results.</terms:description>
        <terms:title>DQA : Data Quality Assessment Ontology</terms:title>
        <vann:preferredNamespacePrefix>dqa</vann:preferredNamespacePrefix>
        <vann:preferredNamespaceUri>http://www.semanticweb.org/dqa</vann:preferredNamespaceUri>
    </owl:Ontology>
    


    <!-- 
    ///////////////////////////////////////////////////////////////////////////////////////
    //
    // Object Properties
    //
    ///////////////////////////////////////////////////////////////////////////////////////
     -->

    


    <!-- http://www.example.org/dqa#assessesIndicator -->

    <owl:ObjectProperty rdf:about="http://www.example.org/dqa#assessesIndicator">
        <rdfs:domain rdf:resource="http://www.example.org/dqa#QualityAssessmentProcess"/>
        <rdfs:range rdf:resource="http://www.w3.org/ns/dqv#Dimension"/>
        <rdfs:comment xml:lang="en">Establishes a relationship between a quality assessment process and the specific indicator it evaluates.</rdfs:comment>
        <rdfs:label xml:lang="en">assessesIndicator</rdfs:label>
    </owl:ObjectProperty>
    


    <!-- http://www.example.org/dqa#hasGranularity -->

    <owl:ObjectProperty rdf:about="http://www.example.org/dqa#hasGranularity">
        <rdfs:domain rdf:resource="http://www.example.org/dqa#QualityAssessmentProcess"/>
        <rdfs:range rdf:resource="http://www.example.org/dqa#AssessmentGranularity"/>
        <rdfs:comment xml:lang="en">Specifies the level of granularity at which data quality is assessed, either at the unique observation level or for a set of observations.</rdfs:comment>
        <rdfs:label xml:lang="en">hasGranularity</rdfs:label>
    </owl:ObjectProperty>
    


    <!-- http://www.example.org/dqa#hasLabel -->

    <owl:ObjectProperty rdf:about="http://www.example.org/dqa#hasLabel">
        <rdfs:domain rdf:resource="http://www.w3.org/ns/dqv#QualityMeasurement"/>
        <rdfs:range rdf:resource="http://www.example.org/dqa#AssessmentLabel"/>
        <rdfs:comment xml:lang="en">Links a quality measurement to an assessment label that categorizes the evaluation result into qualitative labels (e.g., &quot;High Quality&quot;, &quot;Medium Quality&quot;, &quot;Low Quality&quot;). This facilitates the interpretation of numerical quality scores in a more understandable way.</rdfs:comment>
        <rdfs:label xml:lang="en">hasLabel</rdfs:label>
    </owl:ObjectProperty>
    


    <!-- http://www.example.org/dqa#producesResult -->

    <owl:ObjectProperty rdf:about="http://www.example.org/dqa#producesResult">
        <rdfs:domain rdf:resource="http://www.example.org/dqa#QualityAssessmentProcess"/>
        <rdfs:range rdf:resource="http://www.w3.org/ns/dqv#QualityMeasurement"/>
        <rdfs:comment xml:lang="en">Associates a quality assessment process with its resulting evaluation, providing insight into data quality outcomes.</rdfs:comment>
        <rdfs:label xml:lang="en">producesResult</rdfs:label>
    </owl:ObjectProperty>
    


    <!-- http://www.example.org/dqa#usesMethod -->

    <owl:ObjectProperty rdf:about="http://www.example.org/dqa#usesMethod">
        <rdfs:domain rdf:resource="http://www.example.org/dqa#QualityAssessmentProcess"/>
        <rdfs:range rdf:resource="http://www.example.org/dqa#AssessmentMethod"/>
        <rdfs:comment xml:lang="en">Links a quality assessment process to the specific method used for evaluation, either formula-based or path-based methods.</rdfs:comment>
        <rdfs:label xml:lang="en">usesMethod</rdfs:label>
    </owl:ObjectProperty>
    


    <!-- http://www.example.org/dqa#usesMetric -->

    <owl:ObjectProperty rdf:about="http://www.example.org/dqa#usesMetric">
        <rdfs:domain rdf:resource="http://www.example.org/dqa#FormulaBasedMethod"/>
        <rdfs:range rdf:resource="http://www.w3.org/ns/dqv#Metric"/>
        <rdfs:comment xml:lang="en">Defines the metric employed by a particular assessment method to measure data quality.</rdfs:comment>
        <rdfs:label xml:lang="en">usesMetric</rdfs:label>
    </owl:ObjectProperty>
    


    <!-- 
    ///////////////////////////////////////////////////////////////////////////////////////
    //
    // Data properties
    //
    ///////////////////////////////////////////////////////////////////////////////////////
     -->

    


    <!-- http://www.example.org/dqa#labelThreshold -->

    <owl:DatatypeProperty rdf:about="http://www.example.org/dqa#labelThreshold">
        <rdfs:range rdf:resource="http://www.w3.org/2001/XMLSchema#float"/>
        <rdfs:comment xml:lang="en">Associates an assessment label with a numerical threshold that defines the boundary for assigning a specific quality category. e.g.  if the threshold for &quot;High Quality&quot; is 80%, then a quality measurement with a result above this value will be labeled accordingly.</rdfs:comment>
        <rdfs:label xml:lang="en">labelThreshold</rdfs:label>
    </owl:DatatypeProperty>
    


    <!-- 
    ///////////////////////////////////////////////////////////////////////////////////////
    //
    // Classes
    //
    ///////////////////////////////////////////////////////////////////////////////////////
     -->

    


    <!-- http://www.example.org/dqa#AssessmentGranularity -->

    <owl:Class rdf:about="http://www.example.org/dqa#AssessmentGranularity">
        <rdfs:comment xml:lang="en">Represents the level at which data quality is assessed.</rdfs:comment>
        <rdfs:label xml:lang="en">AssessmentGranularity</rdfs:label>
    </owl:Class>
    


    <!-- http://www.example.org/dqa#AssessmentLabel -->

    <owl:Class rdf:about="http://www.example.org/dqa#AssessmentLabel">
        <rdfs:comment xml:lang="en">Tag used to represent the qualitative result of a quality evaluation. It links a numerical quality measurement to a human-readable label, such as &quot;High Quality,&quot; &quot;Medium Quality,&quot; or &quot;Low Quality.&quot;</rdfs:comment>
        <rdfs:label xml:lang="en">AssessmentLabel</rdfs:label>
    </owl:Class>
    


    <!-- http://www.example.org/dqa#AssessmentMethod -->

    <owl:Class rdf:about="http://www.example.org/dqa#AssessmentMethod">
        <rdfs:comment xml:lang="en">Defines the specific method applied to assess data quality, it is eaither a formula-based or path-based evaluation approach.</rdfs:comment>
        <rdfs:label xml:lang="en">AssessmentMethod</rdfs:label>
    </owl:Class>
    


    <!-- http://www.example.org/dqa#FormulaBasedMethod -->

    <owl:Class rdf:about="http://www.example.org/dqa#FormulaBasedMethod">
        <rdfs:subClassOf rdf:resource="http://www.example.org/dqa#AssessmentMethod"/>
        <rdfs:comment xml:lang="en">A quality assessment method that evaluates data quality using a predefined mathematical formula.</rdfs:comment>
        <rdfs:comment xml:lang="en">FormulaBasedMethod</rdfs:comment>
    </owl:Class>
    


    <!-- http://www.example.org/dqa#GranularitySetObservation -->

    <owl:Class rdf:about="http://www.example.org/dqa#GranularitySetObservation">
        <rdfs:subClassOf rdf:resource="http://www.example.org/dqa#AssessmentGranularity"/>
        <rdfs:comment xml:lang="en">A granularity level focusing on the quality assessment of sets of observations.</rdfs:comment>
        <rdfs:label xml:lang="en">GranularitySetObservation</rdfs:label>
    </owl:Class>
    


    <!-- http://www.example.org/dqa#GranularityUniqueObservation -->

    <owl:Class rdf:about="http://www.example.org/dqa#GranularityUniqueObservation">
        <rdfs:subClassOf rdf:resource="http://www.example.org/dqa#AssessmentGranularity"/>
        <rdfs:comment xml:lang="en">A granularity level focusing on the quality assessment of individual.</rdfs:comment>
        <rdfs:label xml:lang="en">GranularityUniqueObservation</rdfs:label>
    </owl:Class>
    


    <!-- http://www.example.org/dqa#PathBasedMethod -->

    <owl:Class rdf:about="http://www.example.org/dqa#PathBasedMethod">
        <rdfs:subClassOf rdf:resource="http://www.example.org/dqa#AssessmentMethod"/>
        <rdfs:comment xml:lang="en">A method that assesses data quality based on considering the path through which the data was generated and transmitted (e.g. provenance ..)</rdfs:comment>
        <rdfs:label xml:lang="en">PathBasedMethod</rdfs:label>
    </owl:Class>
    


    <!-- http://www.example.org/dqa#QualityAssessmentProcess -->

    <owl:Class rdf:about="http://www.example.org/dqa#QualityAssessmentProcess">
        <rdfs:comment xml:lang="en">Represents the overall process of assessing data quality.</rdfs:comment>
        <rdfs:label xml:lang="en">QualityAssessmentProcess</rdfs:label>
    </owl:Class>
    


    <!-- http://www.example.org/dqa#SetObservationMultipleDevice -->

    <owl:Class rdf:about="http://www.example.org/dqa#SetObservationMultipleDevice">
        <rdfs:subClassOf rdf:resource="http://www.example.org/dqa#GranularitySetObservation"/>
        <rdfs:label xml:lang="en">SetObservationMultipleDevice</rdfs:label>
    </owl:Class>
    


    <!-- http://www.example.org/dqa#SetObservationSingleDevice -->

    <owl:Class rdf:about="http://www.example.org/dqa#SetObservationSingleDevice">
        <rdfs:subClassOf rdf:resource="http://www.example.org/dqa#GranularitySetObservation"/>
        <rdfs:label xml:lang="en">SetObservationSingleDevice</rdfs:label>
    </owl:Class>
</rdf:RDF>



<!-- Generated by the OWL API (version 4.5.29.2024-05-13T12:11:03Z) https://github.com/owlcs/owlapi -->

